core/Result.v
@@ -1,0 +1,30 @@
+Require Import Coq.Lists.List.
+Require Import Hammer.Plugin.Hammer.
+
+(* Consider a Prop P. We want to know if P holds but we don't have a decision procedure.
+  So we use a tactic to construct a sumbool {P} + {True}, which stands either we prove P
+  or we failed to prove P. *)
+
+Definition result (P : Prop) : Type := {P} + {True}.
+
+Module Result.
+
+Definition and {P Q} (r1 : result P) (r2 : result Q) : result (P /\ Q) :=
+  match r1, r2 with
+  | left r1, left r2 =>
+      left (conj r1 r2)
+  | _, _ =>
+      right I
+  end.
+
+Definition or {P Q} (r1 : result P) (r2 : result Q) : result (P \/ Q) :=
+  match r1, r2 with
+  | left r1, _ =>
+      left (or_introl r1)
+  | _, left r2 =>
+      left (or_intror r2)
+  | _, _ =>
+      right I
+  end.
+
+End Result.
